proving CompileFunc.v

platform/cito/CompileFunc.v
@@ -10,21 +10,23 @@ Section TopSection.
 
   Require Import List.
   Require Import WellFormed.
-  Record GoodFunc := 
+  Record GoodFunc f := 
     {
-      NoDupVars : NoDup (ArgVars func ++ Vars func);
-      WellFormed : wellformed (Body func)
+      NoDupVars : NoDup (ArgVars f ++ LocalVars f);
+      WellFormed : wellformed (Body f)
     }.
 
-  Hypothesis good_func : GoodFunc.
+  Hypothesis good_func : GoodFunc func.
 
-  Variable optimizer : Stmt -> Stmt.
+  Definition Optimizer := Stmt -> Stmt.
 
-  Definition GoodOptimizer : Prop.
+  Variable optimizer : Optimizer.
+
+  Definition GoodOptimizer : Optimizer -> Prop.
     admit.
   Qed.
 
-  Hypothesis good_optimizer : GoodOptimizer.
+  Hypothesis good_optimizer : GoodOptimizer optimizer.
 
   Require Import Inv.
   Require Import Malloc.
@@ -48,82 +50,283 @@ Section TopSection.
 
   Section Body.
 
-    Variable imports : LabelMap.t assert.
+  Variable imports : LabelMap.t assert.
 
-    Variable imports_global : importsGlobal imports.
+  Variable imports_global : importsGlobal imports.
 
-    Definition stack_slot n := LvMem (Sp + (4 * n)%nat)%loc.
+  Definition stack_slot n := LvMem (Sp + (4 * n)%nat)%loc.
 
-    Definition Seq2 := @Seq_ _ imports_global module_name.
+  Definition Seq2 := @Seq_ _ imports_global module_name.
 
-    Definition Skip := Skip_ imports module_name.
+  Definition Skip := Skip_ imports module_name.
 
-    Fixpoint Seq ls :=
-      match ls with
-        | nil => Skip
-        | a :: ls' => Seq2 a (Seq ls')
+  Fixpoint Seq ls :=
+    match ls with
+      | nil => Skip
+      | a :: ls' => Seq2 a (Seq ls')
+    end.
+
+  Definition Strline := Straightline_ imports module_name.
+
+  Definition CheckExtraStack (n : nat) cmd :=
+    Seq2 
+      (Strline (IL.Assign Rv (stack_slot 1) :: nil))
+      (Structured.If_ imports_global n Le Rv cmd
+                      (Diverge_ imports module_name)).
+
+  Definition vars := SyntaxFunc.ArgVars func ++ LocalVars func.
+
+  Require Import Depth.
+  Definition temp_size := depth (SyntaxFunc.Body func).
+
+  Require CompileStmt.
+  Definition compile_stmt s := CompileStmt.compile vars temp_size imports_global module_name s Syntax.Skip.
+
+  Definition body_stmt := optimizer (SyntaxFunc.Body func).
+
+  Infix "/\" := cons : tmp_scope.
+  Open Scope tmp_scope.
+  Definition body' :=
+    let stack_needed := length (LocalVars func) + temp_size in
+    CheckExtraStack 
+      stack_needed
+      (Seq
+         (Strline 
+            (Binop (stack_slot 1) (stack_slot 1) Minus stack_needed /\
+             Assign (stack_slot 0) Rp /\ nil) /\
+          compile_stmt body_stmt /\
+          Strline 
+            (Assign Rp (stack_slot 0) /\ nil) /\
+          IGoto _ _ Rp /\ nil)).
+  Close Scope tmp_scope.
+
+  Definition imply (pre new_pre: assert) := forall specs x, interp specs (pre x) -> interp specs (new_pre x).
+
+  Definition verifCond pre := imply pre spec :: nil.
+
+  Require Import Wrap.
+
+  Lemma verifCond_ok : forall pre : assert, vcs (verifCond pre) -> vcs (VerifCond (body' pre)).
+  Proof.
+    Opaque funcs_ok.
+    Opaque mult.
+
+    Require Import WordFacts.
+    Require Import CompileStmtTactics.
+    Require Import Arith.
+
+    Open Scope nat.
+
+    Set Printing Coercions.
+
+    unfold verifCond, imply; wrap0.
+
+    Focus 4.
+    (* vc 4 *)
+    unfold CompileStmtSpec.imply in *.
+    unfold CompileStmtSpec.precond in *.
+    post.
+    eapply H2 in H0.
+    unfold spec in *.
+    unfold inv in *.
+    unfold inv_template in *.
+    unfold is_state in *.
+    unfold has_extra_stack in *.
+    unfold stack_slot in *.
+    post.
+    match goal with
+      | H : length _ = 0 |- _ => rewrite H in *
+    end.
+    rewrite plus_0_r in *.
+    rewrite fold_4_mult_1 in *.
+    rewrite mult_0_r in *.
+    destruct_state.
+    hiding ltac:(evaluate auto_ext).
+    fold (@length string) in *.
+    rewrite_natToW_plus.
+    repeat rewrite wplus_assoc in *.
+    Lemma GoodFunc_goodSize : forall f, GoodFunc f -> goodSize (length (LocalVars f) + depth (SyntaxFunc.Body f)).
+      admit.
+    Qed.
+
+    Ltac gen_le :=
+      match goal with
+        | H : (natToW ?a ^+ natToW ?b <= natToW ?c)%word |- _ => assert (a + b <= c) by (eapply wle_goodSize_le; [rewrite_natToW_plus | eapply GoodFunc_goodSize]; eauto); assert (a <= c) by omega; assert (b <= c - a) by omega
       end.
 
-    Definition Strline := Straightline_ imports module_name.
+    gen_le.
+    Require Import SepHints2.
+    set (len_args := length (SyntaxFunc.ArgVars func)) in *.
+    set (w := Regs x1 _ ^+ _ ^+ _) in *.
+    set (len_local := length (LocalVars func)) in *.
+    replace (w =?> x7)%Sep with (buf_to_split w x7 len_local) in * by (unfold buf_to_split; eauto).
+    assert (buf_splittable x7 len_local) by (unfold buf_splittable; eauto).
+    Require Import SepHints5.
+    hiding ltac:(evaluate hints_split_buf).
+    rewrite fold_4_mult in *.
 
-    Definition CheckExtraStack (n : nat) cmd :=
-      Seq2 
-        (Strline (IL.Assign Rv (stack_slot 1) :: nil))
-        (Structured.If_ imports_global n Le Rv cmd
-                        (Diverge_ imports module_name)).
+    unfold_all.
+    set (w := Regs x1 _ ^+ _ ^+ _ ^+ _) in *.
+    set (buf := x7 - _) in *.
+    replace (w =?> buf)%Sep with (buf_to_split w buf temp_size) in * by (unfold buf_to_split; eauto).
+    assert (buf_splittable buf temp_size) by (unfold buf_splittable; eauto).
+    hiding ltac:(evaluate hints_split_buf).
+    fold (@length string) in *.
+    rewrite fold_4_mult in *.
+    Definition to_intro_array (_ : W) := True.
 
-    Definition vars := SyntaxFunc.ArgVars func ++ Vars func.
-
-    Require Import Depth.
-    Definition temp_size := depth (SyntaxFunc.Body func).
-
-    Require CompileStmt.
-    Definition compile_stmt s := CompileStmt.compile vars temp_size imports_global module_name s Syntax.Skip.
-
-    Infix "/\" := cons : tmp_scope.
-    Open Scope tmp_scope.
-    Definition body' :=
-      let stack_needed := length (Vars func) + temp_size in
-      CheckExtraStack 
-        stack_needed
-        (Seq
-           (Strline 
-              (Binop (stack_slot 1) (stack_slot 1) Minus stack_needed /\
-               Assign (stack_slot 0) Rp /\ nil) /\
-            compile_stmt (optimizer (SyntaxFunc.Body func)) /\
-            Strline 
-              (Assign Rp (stack_slot 0) /\ nil) /\
-            IGoto _ _ Rp /\ nil)).
-    Close Scope tmp_scope.
-
-    Definition imply (pre new_pre: assert) := forall specs x, interp specs (pre x) -> interp specs (new_pre x).
-
-    Definition verifCond pre := imply pre spec :: nil.
-
-    Require Import Wrap.
-    Definition body : cmd imports module_name.
-      refine (
-          Wrap imports imports_global module_name 
-               body'
-               (fun pre => Postcondition (body' pre))
-               verifCond
-               _ _).
-      wrap0.
-      unfold verifCond, imply; wrap0.
-      eapply H2 in H.
-      unfold spec in *.
-      unfold inv in *.
-      unfold inv_template in *.
-      Opaque funcs_ok.
-      post.
+    Lemma intro_array : forall len p, to_intro_array p -> p =?> len ===> Ex ls, [| length ls = len |] * array ls p.
       admit.
-      admit.
-      admit.
-      admit.
-      admit.
-      admit.
-      admit.
+    Qed.
+
+    Definition hints_intro_array : TacPackage.
+      prepare intro_array tt.
     Defined.
+
+    assert (to_intro_array w) by (unfold to_intro_array; eauto).
+    hiding ltac:(evaluate hints_intro_array).
+    fold (@length string) in *.
+
+    set (p_local_vars := Regs x1 _ ^+ _ ^+ _) in *.
+    assert (to_intro_array p_local_vars) by (unfold to_intro_array; eauto).
+    hiding ltac:(evaluate hints_intro_array).
+    fold (@length string) in *.
+
+    Lemma GoodFunc_NoDup_LocalVars : forall f, GoodFunc f -> NoDup (LocalVars f).
+      admit.
+    Qed.
+    
+    Require Import SepHints3.
+    set (lvars := LocalVars _) in *.
+    rewrite (@replace_array_to_locals x4 _ lvars) in H20.
+    assert (array_to_locals_ok x4 lvars) by (unfold_all; unfold array_to_locals_ok; descend; eapply GoodFunc_NoDup_LocalVars; eauto).
+    hiding ltac:(evaluate hints_array_to_locals).
+
+    unfold_all.
+    unfold vars in *.
+    set (extra := _ - _ - _) in *.
+    descend.
+    eauto.
+    match goal with
+      | H : _ = Regs x1 Sp |- _ => rewrite H in *
+    end.
+    instantiate (6 := (_, _)); simpl.
+    instantiate (7 := x).
+    match goal with
+      | H : _ = temp_size |- _ => rewrite H in *
+    end.
+    instantiate (3 := extra).
+    repeat rewrite app_length in *.
+    repeat rewrite Mult.mult_plus_distr_l in *.
+    rewrite_natToW_plus.
+    repeat rewrite natToW_plus.
+    repeat rewrite wplus_assoc in *.
+
+    Lemma minus_plus_two : forall a b c, a - (b + c) = a - b - c.
+      intros; omega.
+    Qed.
+
+    replace (natToW _ ^- _) with (natToW extra) in * by (unfold_all; rewrite <- minus_plus_two; rewrite natToW_minus; [rewrite natToW_plus | ]; eauto).
+
+    generalize H20; clear_all; intros.
+
+    repeat hiding ltac:(step auto_ext).
+
+    fold (@length string) in *.
+    fold (@app string) in *.
+
+    Definition combined_locals vars1 vars2 vs1 vs2 p  := locals (vars1 ++ vars2) (merge vs1 vs2 vars1) 0 p.
+
+    Definition locals_combinable A (vars vars2 : list A) := NoDup (vars ++ vars2).
+
+    Lemma combine_locals : forall vars1 vars2 vs1 vs2 p, locals vars1 vs1 0 p * locals vars2 vs2 0 (p ^+ $(4 * length vars1)) ===> combined_locals vars1 vars2 vs1 vs2 p.
+      admit.
+    Qed.
+
+    Definition hints_combine_locals : TacPackage.
+      prepare tt combine_locals.
+    Defined.
+
+    instantiate (1 := merge v x9 (SyntaxFunc.ArgVars func)).
+    set (avars := SyntaxFunc.ArgVars _) in *.
+    set (lvars := SyntaxFunc.LocalVars _) in *.
+    rewrite wplus_0 in *.
+    set (w := Regs _ _ ^+ natToW 8) in *.
+    Lemma fold_combined_locals : forall vars1 vars2 vs1 vs2 p, locals (vars1 ++ vars2) (merge vs1 vs2 vars1) 0 p = combined_locals vars1 vars2 vs1 vs2 p.
+      eauto.
+    Qed.
+
+    rewrite fold_combined_locals.
+
+    assert (locals_combinable avars lvars).
+    unfold locals_combinable.
+    Lemma GoodFunc_NoDup_vars : forall f, GoodFunc f -> NoDup (SyntaxFunc.ArgVars f ++ LocalVars f).
+      admit.
+    Qed.
+
+    eapply GoodFunc_NoDup_vars; eauto.
+    admit.
+
+    repeat hiding ltac:(step hints_combine_locals).
+    (*here*)
+
+
+    (* vc 1 *)
+    eapply H2 in H.
+    unfold spec in *.
+    unfold inv in *.
+    unfold inv_template in *.
+    unfold is_state in *.
+    unfold has_extra_stack in *.
+    unfold stack_slot in *.
+    rewrite fold_4_mult_1 in *.
+    post.
+    hiding ltac:(evaluate auto_ext).
+
+    (* vc 2 *)
+    eapply H2 in H1.
+    unfold spec in *.
+    unfold inv in *.
+    unfold inv_template in *.
+    unfold is_state in *.
+    unfold has_extra_stack in *.
+    unfold stack_slot in *.
+    rewrite fold_4_mult_1 in *.
+    post.
+    hiding ltac:(evaluate auto_ext).
+
+    (* vc 3 *)
+    eapply H2 in H1.
+    unfold spec in *.
+    unfold inv in *.
+    unfold inv_template in *.
+    unfold is_state in *.
+    unfold has_extra_stack in *.
+    unfold stack_slot in *.
+    post.
+    rewrite fold_4_mult_1 in *.
+    rewrite mult_0_r in *.
+    hiding ltac:(evaluate auto_ext).
+
+    admit.
+    admit.
+    admit.
+    admit.
+    admit.
+    admit.
+    admit.
+  Qed.
+
+  Definition body : cmd imports module_name.
+    refine (
+        Wrap imports imports_global module_name 
+             body'
+             (fun pre => Postcondition (body' pre))
+             verifCond
+             _ _).
+    wrap0.
+    eapply verifCond_ok.
+  Defined.
 
   End Body.
 
